Progress on the symboltablegen proof. The code compiles again.

x86/RelocProgSemantics.v
@@ -161,7 +161,7 @@ Definition eval_ros (ge : Genv.t) (ros : ireg + ident) (rs : regset) :=
   end.
 
 
-Definition goto_ofs (ge: Genv.t) (sz:ptrofs) (ofs:Z) (rs: regset) (m: mem) :=
+Definition goto_ofs (sz:ptrofs) (ofs:Z) (rs: regset) (m: mem) :=
   match rs#PC with
   | Vptr b o =>
     Next (rs#PC <- (Vptr b (Ptrofs.add o (Ptrofs.add sz (Ptrofs.repr ofs))))) m
@@ -466,20 +466,20 @@ Definition exec_instr (ge: Genv.t) (i: instruction) (rs: regset) (m: mem) : outc
       Next (nextinstr_nf (rs#rd <- (Vsingle Float32.zero)) sz) m
   (** Branches and calls *)
   | Pjmp_l_rel ofs =>
-      goto_ofs ge sz ofs rs m
+      goto_ofs sz ofs rs m
   | Pjmp (inr id) sg =>
       Next (rs#PC <- (Genv.symbol_address ge id Ptrofs.zero)) m
   | Pjmp (inl r) sg =>
       Next (rs#PC <- (rs r)) m
   | Pjcc_rel cond ofs =>
       match eval_testcond cond rs with
-      | Some true => goto_ofs ge sz ofs rs m
+      | Some true => goto_ofs sz ofs rs m
       | Some false => Next (nextinstr rs sz) m
       | None => Stuck
       end
   | Pjcc2_rel cond1 cond2 ofs =>
       match eval_testcond cond1 rs, eval_testcond cond2 rs with
-      | Some true, Some true => goto_ofs ge sz ofs rs m
+      | Some true, Some true => goto_ofs sz ofs rs m
       | Some _, Some _ => Next (nextinstr rs sz) m
       | _, _ => Stuck
       end
@@ -488,7 +488,7 @@ Definition exec_instr (ge: Genv.t) (i: instruction) (rs: regset) (m: mem) : outc
       | Vint n =>
           match list_nth_z tbl (Int.unsigned n) with
           | None => Stuck
-          | Some ofs => goto_ofs ge sz ofs (rs #RAX <- Vundef #RDX <- Vundef) m
+          | Some ofs => goto_ofs sz ofs (rs #RAX <- Vundef #RDX <- Vundef) m
           end
       | _ => Stuck
       end
