x86/Symbtablegen.v
@@ -238,44 +238,48 @@ Proof.
   - simpl. auto.
 Qed.
     
-Definition is_local_jmp (i: instruction) := 
+Definition instr_invalid (i: instruction) := 
   match i with
   | Pjmp_l _ 
   | Pjcc _ _ 
   | Pjcc2 _ _ _ 
-  | Pjmptbl _ _ => True
+  | Pjmptbl _ _ 
+  | Pallocframe _ _ _ 
+  | Pfreeframe _ _ 
+  | Pload_parent_pointer _ _ => True
   | _ => False
   end.
 
-Definition is_not_local_jmp i := ~is_local_jmp i.
+Definition instr_valid i := ~instr_invalid i.
 
-Lemma is_local_jmp_dec: forall i, {is_local_jmp i} + {~is_local_jmp i}.
+Lemma instr_invalid_dec: forall i, {instr_invalid i} + {~instr_invalid i}.
 Proof.
   destruct i; cbn; auto.
 Qed.
 
-Lemma is_not_local_jmp_dec: forall i, {is_not_local_jmp i} + {~is_not_local_jmp i}.
+Lemma instr_valid_dec: forall i, {instr_valid i} + {~instr_valid i}.
 Proof.
-  unfold is_not_local_jmp.
+  unfold instr_valid.
   destruct i; cbn; auto.
 Qed.
 
-Definition def_no_local_jmp (def: option (globdef fundef unit)) :=
+Definition def_instrs_valid (def: option (globdef fundef unit)) :=
   match def with
   | None => True
   | Some (Gvar v) => True
   | Some (Gfun f) =>
     match f with
     | External _ => True
-    | Internal f =>    Forall is_not_local_jmp (fn_code f)
+    | Internal f =>  Forall instr_valid (fn_code f)
     end
   end.
 
-Lemma def_no_local_jmp_dec: forall def, {def_no_local_jmp def} + {~def_no_local_jmp def}.
+Lemma def_instrs_valid_dec: 
+  forall def, {def_instrs_valid def} + {~def_instrs_valid def}.
 Proof.
   destruct def. destruct g.
   - destruct f. 
-    + simpl. apply Forall_dec. apply is_not_local_jmp_dec.
+    + simpl. apply Forall_dec. apply instr_valid_dec.
     + simpl. auto.
   - simpl. auto.
   - simpl. auto.
@@ -286,7 +290,7 @@ Record wf_prog (p:Asm.program) : Prop :=
     wf_prog_norepet_defs: list_norepet (map fst (AST.prog_defs p));
     wf_prog_main_exists: main_exists (AST.prog_main p) (AST.prog_defs p);
     wf_prog_defs_aligned: Forall def_aligned (map snd (AST.prog_defs p));
-    wf_prog_no_local_jmps: Forall def_no_local_jmp (map snd (AST.prog_defs p));
+    wf_prog_no_local_jmps: Forall def_instrs_valid (map snd (AST.prog_defs p));
   }.
 
 Definition check_wellformedness p : { wf_prog p } + { ~ wf_prog p }.
@@ -294,7 +298,7 @@ Proof.
   destruct (list_norepet_dec ident_eq (map fst (AST.prog_defs p))).
   destruct (main_exists_dec (AST.prog_main p) (AST.prog_defs p)).
   destruct (Forall_dec _ def_aligned_dec (map snd (AST.prog_defs p))).
-  destruct (Forall_dec _ def_no_local_jmp_dec (map snd (AST.prog_defs p))).
+  destruct (Forall_dec _ def_instrs_valid_dec (map snd (AST.prog_defs p))).
   left; constructor; auto.
   right. inversion 1. apply n. auto.
   right. inversion 1. apply n. auto.
